Finish subst_lemma for normalization Show that there exists an instantiation for R

2016/Normalization.thy
@@ -20,13 +20,17 @@ fun subst_L :: "nat \<Rightarrow> lterm \<Rightarrow> lterm \<Rightarrow> lterm"
   "subst_L j s ValA = ValA" |
   "subst_L j s (LApp t1 t2) = LApp (subst_L j s t1) (subst_L j s t2)" |
   "subst_L j s (LVar k) = (if k = j then s else LVar k)" |
-  "subst_L j s (LAbs T t) = LAbs T (subst_L (Suc j) s t)"
+  "subst_L j s (LAbs T t) = LAbs T (subst_L (Suc j) (shift_L 1 0 s) t)"
 
 fun FV ::"lterm \<Rightarrow> nat set" where
   "FV (LVar k) = {k}"|
   "FV (LApp t1 t2) = FV t1 \<union> FV t2"|
   "FV (LAbs T t) =  image (\<lambda>x. x - 1) (FV t - {0})" |
   "FV ValA = {}"
+
+inductive is_value_L:: "lterm \<Rightarrow> bool" where
+  "is_value_L ValA" 
+| "is_value_L (LAbs T t)"
 
 inductive eval1_L :: "lterm \<Rightarrow> lterm \<Rightarrow> bool" where
    -- "Rules relating to the evaluation of function application"
@@ -65,52 +69,118 @@ inductive has_type_L :: "lcontext \<Rightarrow> lterm \<Rightarrow> ltype \<Righ
   has_type_LApp:
     "\<Gamma> \<turnstile> t1 |:| (T11 \<rightarrow> T12) \<Longrightarrow> \<Gamma> \<turnstile> t2 |:| T11 \<Longrightarrow> \<Gamma> \<turnstile> LApp t1 t2 |:| T12"
 
-inductive is_value_L:: "lterm \<Rightarrow> bool" where
-  "is_value_L ValA" 
-| "is_value_L (LAbs T t)"
-
-abbreviation R:: " lterm \<Rightarrow> ltype \<Rightarrow> bool" ("(_) \<in>\<^sub>R (_)" [100,100] 200) where
-  "t \<in>\<^sub>R T \<equiv> (\<emptyset> \<turnstile> t |:| T \<and> FV t = {})"
+abbreviation closed ::"lterm \<Rightarrow> bool" where
+  "closed t \<equiv> FV t={}"
 
 abbreviation halts :: "lterm \<Rightarrow> bool" where
-  "halts t \<equiv> \<exists>t'. star eval1_L t t' \<and> (\<forall>t1. \<not> eval1_L t' t1)"
+  "halts t \<equiv> (\<exists>t'. star eval1_L t t' \<and> (\<forall>t1. \<not> eval1_L t' t1)) \<or> (\<forall>t1. \<not> eval1_L t t1)"
 
-lemma R_def:
-  "t \<in>\<^sub>R A = (halts t)"
-  "s \<in>\<^sub>R (T1\<rightarrow>T2) = (\<forall>t. t \<in>\<^sub>R (T1) \<longrightarrow> (LApp s t) \<in>\<^sub>R T2)"
-proof -
-  have lr:"t \<in>\<^sub>R A \<Longrightarrow> halts t"
-    proof -
-      assume H:"t \<in>\<^sub>R A"
-      obtain \<Gamma> where G:"\<Gamma> = \<emptyset>" "\<Gamma> \<turnstile> t |:| A"
-        using H
-        by metis
-      show "halts t"
-        using G(2,1)
-              H[THEN conjunct2] 
-        proof (induction rule:has_type_L.induct)
-          case (has_type_LApp \<Gamma> t1 T1 T2 t2)
-            note hyps=this and FVt1=this(6)[simplified, THEN conjunct1] and
-                 FVt2 = this(6)[simplified, THEN conjunct2]
-            obtain t1' t2' where Ht1:"star eval1_L t1 t1'" "(\<forall>t1. \<not> eval1_L t1' t1)"
-                             and Ht2: " star eval1_L t2 t2' \<and> (\<forall>t1. \<not> eval1_L t2' t1)"
-              using hyps(3)[OF hyps(5) FVt1]
-                    hyps(4)[OF hyps(5) FVt2]
-              by blast
-            show ?case
-              
-              sorry
-        qed (auto simp: eval1_L.simps[of ValA] eval1_L.simps[of "LAbs _ _"])
-  have "halts t \<Longrightarrow> t \<in>\<^sub>R A"
-  sorry
+locale rel_reasoning =
+  fixes R::"lterm \<Rightarrow> ltype \<Rightarrow> bool" ("(_)\<in>\<^sub>R(_)" [150,150] 200)
+  assumes R\<^sub>A: " halts t = t \<in>\<^sub>R A" and 
+          R_fun: " (halts t \<and>
+            (\<forall>s. s \<in>\<^sub>R T1 \<longrightarrow> (LApp t s) \<in>\<^sub>R T2)) = t \<in>\<^sub>R (T1\<rightarrow>T2)" and
+          R_def: "t\<in>\<^sub>RT \<Longrightarrow> closed t \<and> \<emptyset> \<turnstile> t |:| T"
 
-  with lr show "t \<in>\<^sub>R A = (halts t)" by blast
+lemma (in rel_reasoning) R_halts:
+  "t \<in>\<^sub>R T \<Longrightarrow> halts t"
+by (induction T, insert R\<^sub>A[of t] R_fun[of t], auto)
+
+lemma[simp]: "nat (int x + 1) = Suc x" by simp
+lemma[simp]: "nat (1 + int x) = Suc x" by simp
+lemma[simp]: "nat (int x - 1) = x - 1" by simp
+
+lemma gr_Suc_conv: "Suc x \<le> n \<longleftrightarrow> (\<exists>m. n = Suc m \<and> x \<le> m)"
+  by (cases n) auto
+
+lemma FV_shift:
+  "FV (shift_L (int d) c t) = image (\<lambda>x. if x \<ge> c then x + d else x) (FV t)"
+proof (induction t arbitrary: c rule: lterm.induct)
+  case (LAbs T t)
+  thus ?case  by (auto simp: gr_Suc_conv image_iff) force+
+qed auto
+
+lemma FV_subst:
+  "FV (subst_L n t u) = (if n \<in> FV u then (FV u - {n}) \<union> FV t else FV u)"
+proof (induction u arbitrary: n t rule: lterm.induct)
+  case (LAbs T u)
+  thus ?case 
+    by (auto simp: gr0_conv_Suc image_iff FV_shift[of 1, unfolded int_1],
+        (metis DiffI One_nat_def UnCI diff_Suc_1 empty_iff imageI insert_iff nat.distinct(1))+)
+qed (auto simp: gr0_conv_Suc image_iff FV_shift[of 1, unfolded int_1])
+
+lemma eval_det:
+  "eval1_L t t1 \<Longrightarrow> eval1_L t t2 \<Longrightarrow> t1=t2" sorry
+
+lemma preservation:
+  "\<Gamma>\<turnstile> t|:| T \<Longrightarrow> eval1_L t t' \<Longrightarrow> \<Gamma> \<turnstile> t'|:| T" sorry
+
+
+lemma halting_evalL:
+  "eval1_L t t1 \<Longrightarrow> halts t \<Longrightarrow> halts t1"
+proof (induction rule: eval1_L.induct)
+  case (eval1_LApp1 t1 t1' t2)
+    thus ?case 
+      using star.simps[of "eval1_L" "LApp t1 t2"]
+            eval1_L.intros(1) 
+            eval_det
+      by metis
 next
-  have lr:" s \<in>\<^sub>R (T1\<rightarrow>T2) \<Longrightarrow> (\<forall>t. t \<in>\<^sub>R (T1) \<longrightarrow> (LApp s t) \<in>\<^sub>R T2)" sorry
-  have "(\<forall>t. t \<in>\<^sub>R (T1) \<longrightarrow> (LApp s t) \<in>\<^sub>R T2) \<Longrightarrow> s \<in>\<^sub>R (T1\<rightarrow>T2)" sorry
+  case (eval1_LApp2 v t2 t2')
+    then show ?case 
+      using star.simps[of "eval1_L" "LApp v t2"] eval1_L.intros(2) eval_det
+      by metis
+next
+  case (eval1_LApp_LAbs v T t)
+    thus ?case
+      using star.simps[of "eval1_L" "LApp (LAbs T t) v"] 
+            eval1_L.intros(3) eval_det 
+      by metis
+qed
 
-  with lr show "s \<in>\<^sub>R (T1\<rightarrow>T2) = (\<forall>t. t \<in>\<^sub>R (T1) \<longrightarrow> (LApp s t) \<in>\<^sub>R T2)" by satx
-qed      
+lemma halting_evalR:
+  "eval1_L t t1 \<Longrightarrow> halts t1 \<Longrightarrow> halts t"
+by (induction rule: eval1_L.induct) (metis eval1_L.intros star_trans star_step1)+
 
+theorem halting_eval:
+  "eval1_L t t1 \<Longrightarrow> halts t = halts t1"
+using halting_evalL halting_evalR by blast
+
+
+lemma (in rel_reasoning) eval_preserves_R:
+  "\<Gamma> \<turnstile> t|:|T \<Longrightarrow> eval1_L t t' \<Longrightarrow> t \<in>\<^sub>R T \<Longrightarrow> t'\<in>\<^sub>R T"
+proof (induction T arbitrary: \<Gamma> t t')
+  case (A)
+    then show ?case 
+      using A(3)[unfolded R\<^sub>A[symmetric] halting_eval[OF A(2)]]
+            preservation[of \<emptyset> t A t'] A(2)
+            R\<^sub>A[of t']
+      by auto
+next
+  case (Fun T1 T2)
+    note hyps=this
+    have "(\<forall>s. s\<in>\<^sub>RT1 \<longrightarrow> LApp t' s\<in>\<^sub>RT2)" 
+      using hyps(2)[of \<emptyset>, OF _ eval1_LApp1[OF hyps(4)]]
+            hyps(5)[unfolded R_fun[symmetric], THEN conjunct2]
+            R_def[of "LApp t _" T2]
+      by blast
+    then show ?case
+      using R_fun[of t' T1 T2]
+            hyps(5)[unfolded R_fun[symmetric] halting_eval[OF hyps(4)]]
+      by auto
+qed
+
+abbreviation subst_all:: "lterm list \<Rightarrow> lterm \<Rightarrow> lterm" where
+"subst_all V \<equiv> rec_nat id (\<lambda>i r. r \<circ> (subst_L i (V!i))) (length V)"
+
+lemma (in rel_reasoning) subst_R:
+  "\<Gamma> \<turnstile> t |:| T \<Longrightarrow> length V = length \<Gamma> \<Longrightarrow> (\<And>i. i<length V \<Longrightarrow> (V!i) \<in>\<^sub>R (\<Gamma>!i)) \<Longrightarrow> 
+    subst_all V t \<in>\<^sub>R T"
+sorry
+
+theorem (in rel_reasoning) Normalization:
+  "\<emptyset>\<turnstile> t |:| T \<Longrightarrow> halts t"
+using subst_R[of \<emptyset> t T \<emptyset>] R_halts[of t T]
+by auto  
 
 end
